code/streaming/Hacl.Streaming.Blake2.Params.fsti
@@ -1,0 +1,88 @@
+module Hacl.Streaming.Blake2.Params
+
+module HS = FStar.HyperStack
+module B = LowStar.Buffer
+module G = FStar.Ghost
+
+open FStar.HyperStack.ST
+
+module Spec = Spec.Blake2
+
+inline_for_extraction noextract
+val params (a: Spec.alg) : Type
+
+val footprint (#a: Spec.alg) (h: HS.mem) (p: params a) : GTot B.loc
+
+val freeable (#a: Spec.alg) (h: HS.mem) (p: params a) : GTot prop
+
+val invariant (#a: Spec.alg) (h: HS.mem) (p: params a) : GTot prop
+
+val v (#a: Spec.alg) (h: HS.mem) (p: params a) : GTot (Spec.blake2_params a)
+
+val invariant_loc_in_footprint: #a: Spec.alg -> h:HS.mem -> s:params a -> Lemma
+    (requires (invariant h s))
+    (ensures (B.loc_in (footprint h s) h))
+    [ SMTPat (invariant h s) ]
+
+val frame_invariant: #a: Spec.alg -> l:B.loc -> s: params a -> h0:HS.mem -> h1:HS.mem -> Lemma
+    (requires (
+      invariant h0 s /\
+      B.loc_disjoint l (footprint h0 s) /\
+      B.modifies l h0 h1))
+    (ensures (
+      invariant h1 s /\
+      v h0 s == v h1 s /\
+      footprint h1 s == footprint h0 s))
+    [ SMTPat (invariant h1 s); SMTPat (B.modifies l h0 h1) ]
+
+val frame_freeable: #a: Spec.alg -> l:B.loc -> s:params a -> h0:HS.mem -> h1:HS.mem -> Lemma
+    (requires (
+      invariant h0 s /\
+      freeable h0 s /\
+      B.loc_disjoint l (footprint h0 s) /\
+      B.modifies l h0 h1))
+    (ensures (
+      freeable h1 s))
+    [ SMTPat (freeable h1 s); SMTPat (B.modifies l h0 h1) ]
+
+inline_for_extraction noextract
+val alloca: a: Spec.alg -> StackInline (params a)
+  (requires (fun _ -> True))
+  (ensures (fun h0 s h1 ->
+    invariant h1 s /\
+    B.(modifies loc_none h0 h1) /\
+    B.fresh_loc (footprint h1 s) h0 h1 /\
+    B.(loc_includes (loc_region_only true (HS.get_tip h1)) (footprint h1 s))))
+
+inline_for_extraction noextract
+val create_in: a: Spec.alg -> r:HS.rid -> ST (params a)
+  (requires (fun h0 ->
+    HyperStack.ST.is_eternal_region r))
+  (ensures (fun h0 s h1 ->
+    invariant h1 s /\
+    B.(modifies loc_none h0 h1) /\
+    B.fresh_loc (footprint h1 s) h0 h1 /\
+    B.(loc_includes (loc_region_only true r) (footprint h1 s)) /\
+    freeable h1 s))
+
+inline_for_extraction noextract
+val free: #a: Spec.alg -> s:params a -> ST unit
+    (requires fun h0 ->
+      freeable h0 s /\
+      invariant h0 s)
+    (ensures fun h0 _ h1 ->
+      B.(modifies (footprint h0 s) h0 h1))
+
+inline_for_extraction noextract
+val copy: #a:Spec.alg -> s_src:params a -> s_dst:params a ->
+    Stack unit
+      (requires (fun h0 ->
+        invariant h0 s_src /\
+        invariant h0 s_dst /\
+        B.(loc_disjoint (footprint h0 s_src) (footprint h0 s_dst))))
+      (ensures fun h0 _ h1 ->
+        B.(modifies (footprint h0 s_dst) h0 h1) /\
+        footprint h0 s_dst == footprint h1 s_dst /\
+        (freeable h0 s_dst ==> freeable h1 s_dst) /\
+        invariant h1 s_dst /\
+        v h1 s_dst == v h0 s_src)
